proof/theories/Optimize.v
@@ -53,6 +53,8 @@ Proof.
     try (apply list_eq_dec; apply Nat.eq_dec);
     try (apply list_eq_dec; apply list_eq_dec; apply Nat.eq_dec);
     try (apply list_eq_dec; apply transform_eq_dec);
+    try (apply list_eq_dec; decide equality;
+           (apply field_eq_dec || (apply list_eq_dec; apply transform_eq_dec)));
     try (apply list_eq_dec; apply field_eq_dec);
     try apply field_eq_dec;
     try apply Bool.bool_dec;
